parse derive context input

src/cddl/test/CDDLTest.UseDPE.fst
@@ -459,7 +459,7 @@ ensures is_engine_record e (rel_evercddl_derive_context_engine_record x w)
   let hdr, hdr_sig = destruct_pair_concrete_nest _ _ _ _ _ _;
   trade_emp_hyp_r _ _;
   let hdr = destruct_evercddl_bytes_head _ _ _ _ _;
-  trade_emp_hyp_r_elim _ _ _;
+  // trade_emp_hyp_r_elim _ _ _;
   let hdr_sig = destruct_evercddl_bytes_head _ _ _ _ _;
   let bin = destruct_evercddl_bytes_head _ _ _ _ _;
   let bin_hash = destruct_evercddl_bytes_head _ _ _ _ _;
@@ -560,7 +560,6 @@ ensures is_device_id_csr_ingredients res (rel_evercddl_device_id_csr_ingredients
   let ku = destruct_evercddl_nint_head _ _ _ _ _;
   let version =  destruct_evercddl_nint_head _ _ _ _ _;
   let s_common = destruct_evercddl_tstr_head _ _ _ _ _;
-  trade_emp_hyp_r_elim _ _ _;
   let s_org = destruct_evercddl_tstr_head _ _ _ _ _;
   Trade.Util.assoc_hyp_l _ _ _ _;
   let s_country = destruct_evercddl_tstr_head _ _ _ _ _;
@@ -575,55 +574,557 @@ ensures is_device_id_csr_ingredients res (rel_evercddl_device_id_csr_ingredients
   res
 }
 
-fn extract_derive_context_input_args_data x (w:erased _)
-requires rel_evercddl_derive_context_input_args_data x w
-ensures emp
-{
-  unfold (rel_evercddl_derive_context_input_args_data x w);
-  destruct_rel_fun _ _ _ _ _;
-  admit()
+noeq
+type alias_key_crt_ingredients_t = {
+  version: UInt64.t;
+  serialNumber: slice UInt8.t;
+  i_common: slice UInt8.t;
+  i_org: slice UInt8.t;
+  notBefore: slice UInt8.t;
+  notAfter: slice UInt8.t;
+  s_common: slice UInt8.t;
+  s_org: slice UInt8.t;
+  s_country: slice UInt8.t;
+  ku: UInt64.t;
+  l0_version: UInt64.t
 }
 
-fn extract_devive_context_input_args x (w:erased _)
-requires rel_evercddl_derive_context_input_args x w
-ensures emp
+[@@pulse_unfold]
+unfold
+let is_alias_key_crt_ingredients_core (e:alias_key_crt_ingredients_t) sn c o nb na com org cnt : slprop =
+  rel_slice_of_seq false e.serialNumber sn **
+  rel_slice_of_seq false e.i_common c **
+  rel_slice_of_seq false e.i_org o **
+  rel_slice_of_seq false e.notBefore nb **
+  rel_slice_of_seq false e.notAfter na **
+  rel_slice_of_seq false e.s_common com **
+  rel_slice_of_seq false e.s_org org **
+  rel_slice_of_seq false e.s_country cnt
+
+#push-options "--query_stats"
+fn make_alias_key_crt_ingredients 
+    (version:UInt64.t)
+    serialNumber
+    i_common
+    i_org
+    notBefore
+    notAfter
+    s_common
+    s_org
+    s_country
+    (ku
+     l0_version: UInt64.t)
+requires 
+  rel_slice_of_seq false serialNumber 'n **
+  rel_slice_of_seq false i_common 'c **
+  rel_slice_of_seq false i_org 'o **
+  rel_slice_of_seq false notBefore 'nb **
+  rel_slice_of_seq false notAfter 'na **
+  rel_slice_of_seq false s_common 'com **
+  rel_slice_of_seq false s_org 'org **
+  rel_slice_of_seq false s_country 'cnt
+returns 
+  e:alias_key_crt_ingredients_t
+ensures
+  is_alias_key_crt_ingredients_core e 'n 'c 'o 'nb 'na 'com 'org 'cnt **
+  pure (e == { ku; s_country; s_org; s_common; i_org; i_common; notAfter; notBefore; version; serialNumber; l0_version })
 {
-  unfold (rel_evercddl_derive_context_input_args x w);
-  destruct_rel_fun _ _ _ _ _;
-  // with r0 r1 x y. assert (rel_pair r0 r1 
-  //     (evercddl_derive_context_input_args_pretty_left x)
-  //     (spect_evercddl_derive_context_input_args_pretty_left w)
-  // );
-  destruct_fst _ _ 
-      (evercddl_derive_context_input_args_pretty_left x)
-      (spect_evercddl_derive_context_input_args_pretty_left w)
-      _;
-  destruct_fst _ _ _ _ _;
-  destruct_fst _ _ _ _ _;
-  destruct_fst _ _ _ _ _;
-  destruct_fst _ _ _ _ _;
-  destruct_fst _ _ _ _ _;
-  destruct_fst _ _ _ _ _;
-  destruct_snd _ _ _ _ _;
-  admit()
+  let res = { ku; s_country; s_org; s_common; i_org; i_common; notAfter; notBefore; version; serialNumber; l0_version };
+  rewrite each
+    i_common as res.i_common,
+    i_org as res.i_org,
+    notBefore as res.notBefore,
+    notAfter as res.notAfter,
+    version as res.version,
+    serialNumber as res.serialNumber,
+    l0_version as res.l0_version,
+    ku as res.ku,
+    s_common as res.s_common,
+    s_org as res.s_org,
+    s_country as res.s_country;
+  res
 }
+
+let is_alias_key_crt_ingredients (e:alias_key_crt_ingredients_t) (res:slprop) : slprop =
+  exists* sn c o nb na com org cnt.
+    is_alias_key_crt_ingredients_core e sn c o nb na com org cnt **
+    Trade.trade (is_alias_key_crt_ingredients_core e sn c o nb na com org cnt) res
+
+#push-options "--query_stats --ext nothing"
+fn extract_alias_key_crt_ingredients x (w:erased _)
+requires rel_evercddl_alias_key_crt_ingredients x w
+returns res:alias_key_crt_ingredients_t
+ensures is_alias_key_crt_ingredients res (rel_evercddl_alias_key_crt_ingredients x w)
+{
+  unfold_with_trade (`%rel_evercddl_alias_key_crt_ingredients) (rel_evercddl_alias_key_crt_ingredients x w);
+  destruct_rel_fun _ _ _ _ _;
+  Trade.trade_compose _ _ (rel_evercddl_alias_key_crt_ingredients x w);
+
+  let rest, l0_version = destruct_pair_concrete _ _ _ _ _;
+  let rest, ku = destruct_pair_concrete_nest _ _ _ _ _ _;
+  let rest, country = destruct_pair_concrete_nest _ _ _ _ _ _;
+  let rest, org = destruct_pair_concrete_nest _ _ _ _ _ _;
+  let rest, common = destruct_pair_concrete_nest _ _ _ _ _ _;
+  let rest, notAfter = destruct_pair_concrete_nest _ _ _ _ _ _;
+  let rest, notBefore = destruct_pair_concrete_nest _ _ _ _ _ _;
+  let rest, org = destruct_pair_concrete_nest _ _ _ _ _ _;
+  let rest, common = destruct_pair_concrete_nest _ _ _ _ _ _;
+  let version, serialNumber = destruct_pair_concrete_nest _ _ _ _ _ _;
+
+  trade_emp_hyp_r _ _;
+  let version =  destruct_evercddl_nint_head _ _ _ _ _;
+  let serialNumber =  destruct_evercddl_bytes_head _ _ _ _ _;
+  let i_common =  destruct_evercddl_tstr_head _ _ _ _ _;
+  let i_org =  destruct_evercddl_tstr_head _ _ _ _ _;
+  let notBefore = destruct_evercddl_bytes_head _ _ _ _ _;
+  let notAfter = destruct_evercddl_bytes_head _ _ _ _ _;
+  let s_common =  destruct_evercddl_tstr_head _ _ _ _ _;
+  let s_org =  destruct_evercddl_tstr_head _ _ _ _ _;
+  let s_country =  destruct_evercddl_tstr_head _ _ _ _ _;
+  let ku = destruct_evercddl_nint_head _ _ _ _ _;
+  Trade.Util.assoc_hyp_l _ _ _ _;
+  let l0_version = destruct_evercddl_nint_head _ _ _ _ _;
+
+  let res = make_alias_key_crt_ingredients 
+    version
+    serialNumber
+    i_common
+    i_org
+    notBefore
+    notAfter
+    s_common
+    s_org
+    s_country
+    ku
+    l0_version;
+  slprop_equivs();
+  fold (is_alias_key_crt_ingredients res (rel_evercddl_alias_key_crt_ingredients x w));
+  res
+
+}
+
+
+noeq
+type derive_context_l0_record_t = {
+  fwid: slice UInt8.t;
+  device_id_label: slice UInt8.t;
+  alias_key_label: slice UInt8.t;
+  device_id_csr_ingredients: device_id_csr_ingredients_t;
+  alias_key_crt_ingredients: alias_key_crt_ingredients_t;
+}
+
+[@@pulse_unfold]
+unfold
+let is_derive_context_l0_record_core (e:derive_context_l0_record_t) fid did akl : slprop =
+  rel_slice_of_seq false e.fwid fid **
+  rel_slice_of_seq false e.device_id_label did **
+  rel_slice_of_seq false e.alias_key_label akl
+
+let is_derive_context_l0_record (e:derive_context_l0_record_t) (k:slprop) =
+  exists* fid did akl k1 k2.
+    is_derive_context_l0_record_core e fid did akl **
+    is_device_id_csr_ingredients e.device_id_csr_ingredients k1 **
+    is_alias_key_crt_ingredients e.alias_key_crt_ingredients k2 **
+    Trade.trade (is_derive_context_l0_record_core e fid did akl ** k1 ** k2) k
+
+fn make_derive_context_l0_record
+    fwid device_id_label alias_key_label
+    device_id_csr_ingredients
+    alias_key_crt_ingredients
+requires 
+  rel_slice_of_seq false fwid 'fid **
+  rel_slice_of_seq false device_id_label 'did **
+  rel_slice_of_seq false alias_key_label 'akl **
+  is_device_id_csr_ingredients device_id_csr_ingredients 'k1 **
+  is_alias_key_crt_ingredients alias_key_crt_ingredients 'k2
+returns 
+  e:derive_context_l0_record_t
+ensures
+  is_derive_context_l0_record_core e 'fid 'did 'akl **
+  is_device_id_csr_ingredients e.device_id_csr_ingredients 'k1 **
+  is_alias_key_crt_ingredients e.alias_key_crt_ingredients 'k2 **
+  pure (e == { fwid; device_id_label; alias_key_label; device_id_csr_ingredients; alias_key_crt_ingredients })
+{
+  let res = { fwid; device_id_label; alias_key_label; device_id_csr_ingredients; alias_key_crt_ingredients };
+  rewrite each
+    fwid as res.fwid,
+    device_id_label as res.device_id_label,
+    alias_key_label as res.alias_key_label,
+    device_id_csr_ingredients as res.device_id_csr_ingredients,
+    alias_key_crt_ingredients as res.alias_key_crt_ingredients;
+  res
+}
+
+fn extract_derive_context_l0_record x (w:erased _)
+requires rel_evercddl_derive_context_l0_record x w
+returns res:derive_context_l0_record_t
+ensures is_derive_context_l0_record res (rel_evercddl_derive_context_l0_record x w)
+{
+  unfold_with_trade (`%rel_evercddl_derive_context_l0_record) (rel_evercddl_derive_context_l0_record x w);
+  destruct_rel_fun _ _ _ _ _;
+  Trade.trade_compose _ _ (rel_evercddl_derive_context_l0_record x w);
+
+  let rest, ak_i = destruct_pair_concrete _ _ _ _ _;
+  let rest, did_i = destruct_pair_concrete_nest _ _ _ _ _ _;
+  let rest, akl = destruct_pair_concrete_nest _ _ _ _ _ _;
+  let fwid, did_l = destruct_pair_concrete_nest _ _ _ _ _ _;
+
+  trade_emp_hyp_r _ _;
+
+  let fwid = destruct_evercddl_bytes_head _ _ _ _ _;
+  let device_id_label = destruct_evercddl_bytes_head _ _ _ _ _;
+  let alias_key_label = destruct_evercddl_bytes_head _ _ _ _ _;
+  let device_id_csr_ingredients = extract_device_id_csr_ingredients _ _;
+  Trade.Util.assoc_hyp_l _ _ _ _;
+  let alias_key_crt_ingredients = extract_alias_key_crt_ingredients _ _;
+  let res = make_derive_context_l0_record 
+    fwid
+    device_id_label
+    alias_key_label
+    device_id_csr_ingredients
+    alias_key_crt_ingredients;
+  slprop_equivs();
+  fold (is_derive_context_l0_record res (rel_evercddl_derive_context_l0_record x w));
+  res
+}
+
+fn destruct_rel_either_left 
+    (#a #b #a' #b':Type0) 
+    (r:rel a b)
+    (r':rel a' b')
+    (x:either a a')
+    (y:erased (either b b'))
+    (res:slprop)
+requires 
+  rel_either r r' x y **
+  pure (Inl? x) **
+  Trade.trade (rel_either r r' x y) res
+returns
+  xx:a
+ensures
+  exists* (yy:b).
+    pure (y == Inl yy /\ x == Inl xx) **
+    r xx yy **
+    Trade.trade (r xx yy) res
+{
+  rel_either_cases _ _ _ _;
+  let xx = Inl?.v x;
+  let yy = hide <| Inl?.v y;
+  rewrite each x as (Inl xx);
+  rel_either_eq_left r r' xx yy;
+  Trade.rewrite_with_trade 
+    (rel_either r r' (Inl xx) y)
+    (r xx yy);
+  rewrite each (Inl #a #a' xx) as x;
+  Trade.trade_compose _ _ res;
+  xx
+}
+
+fn destruct_rel_either_right
+    (#a #b #a' #b':Type0) 
+    (r:rel a b)
+    (r':rel a' b')
+    (x:either a a')
+    (y:erased (either b b'))
+    (res:slprop)
+requires 
+  rel_either r r' x y **
+  pure (Inr? x) **
+  Trade.trade (rel_either r r' x y) res
+returns
+  xx:a'
+ensures
+  exists* (yy:b').
+    pure (y == Inr yy /\ x == Inr xx) **
+    r' xx yy **
+    Trade.trade (r' xx yy) res
+{
+  rel_either_cases _ _ _ _;
+  let xx = Inr?.v x;
+  let yy = hide <| Inr?.v y;
+  rewrite each x as (Inr xx);
+  rel_either_eq_right r r' xx yy;
+  Trade.rewrite_with_trade 
+    (rel_either r r' (Inr xx) y)
+    (r' xx yy);
+  rewrite each (Inr #a #a' xx) as x;
+  Trade.trade_compose _ _ res;
+  xx
+}
+
+ghost
+fn is_engine_record_compose (e:engine_record_t) (res res':slprop)
+requires is_engine_record e res ** Trade.trade res res'
+ensures is_engine_record e res'
+{
+  unfold is_engine_record;
+  Trade.trade_compose _ _ res';
+  fold is_engine_record;
+}
+
+ghost
+fn is_derive_context_l0_record_compose e res res'
+requires is_derive_context_l0_record e res ** Trade.trade res res'
+ensures is_derive_context_l0_record e res'
+{
+  unfold is_derive_context_l0_record;
+  Trade.trade_compose _ _ res';
+  fold is_derive_context_l0_record
+}
+
+let is_derive_context_input_args 
+    (e:either engine_record_t derive_context_l0_record_t) 
+    (res:slprop) 
+: slprop
+= match e with
+  | Inl e -> is_engine_record e res
+  | Inr e -> is_derive_context_l0_record e res
+
+fn extract_derive_context_input_args_data x (w:erased _)
+requires rel_evercddl_derive_context_input_args_data x w
+returns e:either engine_record_t derive_context_l0_record_t
+ensures is_derive_context_input_args e (rel_evercddl_derive_context_input_args_data x w)
+{
+  unfold_with_trade (`%rel_evercddl_derive_context_input_args_data) (rel_evercddl_derive_context_input_args_data _ _);
+  destruct_rel_fun _ _ _ _ _;
+  Trade.trade_compose _ _ (rel_evercddl_derive_context_input_args_data x w);
+  rel_either_cases _ _ _ _;
+  match (evercddl_derive_context_input_args_data_pretty_left x) {
+    Inl _ -> {
+      let _ = destruct_rel_either_left _ _ _ _ _;
+      let engine_record = extract_derive_context_engine_record _ _;
+      is_engine_record_compose _ _ _;
+      fold (is_derive_context_input_args (Inl engine_record));
+      Inl engine_record
+    }
+
+    Inr l0 -> {
+      let _ = destruct_rel_either_right _ _ _ _ _;
+      let l0_record = extract_derive_context_l0_record _ _;
+      is_derive_context_l0_record_compose _ _ _;
+      fold (is_derive_context_input_args (Inr l0_record));
+      Inr l0_record
+    }
+  }
+}
+
+ghost
+fn fold_with_trade (s:string) (p:slprop)
+requires my_unfold s p
+ensures p
+{
+  norm_spec [delta_only [s]; hnf; iota; primops] p;
+  rewrite (my_unfold s p) as p;
+}
+
+
+[@@pulse_unfold]
+unfold
+let my_unfold_any (#a:Type) (s:string) (p:a) = norm [delta_only [s]; hnf; iota; primops] p
+
+ghost
+fn fold_last_relation
+   (#a0 #b0 #a1 #b1:Type0)
+   (#r:rel a0 b0)
+   (s:string)
+   (p:rel a1 b1)
+   (#x:_)
+   (#y:_)
+   (#res:slprop)
+requires 
+  rel_pair r (my_unfold_any s p) x y **
+  Trade.trade (rel_pair r (my_unfold_any s p) x y) res
+ensures rel_pair r p x y **   Trade.trade (rel_pair r p x y) res
+{
+  norm_spec [delta_only [s]; hnf; iota; primops] p;
+  rewrite each (my_unfold_any s p) as p;
+}
+
+
+// fn test_fold x y
+// requires
+//  rel_either_left (rel_slice_of_table (mk_eq_test_bij spect_aux_env15_type_1_pretty_right
+//                     spect_aux_env15_type_1_pretty_left
+//                     spect_aux_env15_type_1_pretty_left_right
+//                     spect_aux_env15_type_1_pretty_right_left
+//                     (mk_eq_test_bij spect_evercddl_uint_pretty_right
+//                         spect_evercddl_uint_pretty_left
+//                         spect_evercddl_uint_pretty_left_right
+//                         spect_evercddl_uint_pretty_right_left
+//                         (EqTest.eqtype_eq UInt64.t)))
+//                 rel_aux_env15_type_1
+//                 rel_aux_env15_type_3)
+//             (rel_map_iterator CBOR.Pulse.API.Det.C.cbor_det_match
+//                 CBOR.Pulse.API.Det.C.cbor_det_map_iterator_match
+//                 aux_env15_type_1_pretty
+//                 aux_env15_type_3_pretty
+//                 (CDDL.Pulse.Iterator.Base.mk_spec rel_aux_env15_type_1)
+//                 (CDDL.Pulse.Iterator.Base.mk_spec rel_aux_env15_type_3))
+//                 x y
+// ensures
+//   tstr_any x y
+// {
+//   fold_with_trade (`%tstr_any) (tstr_any x y);
+// }
+
+
+fn fst_pair_concrete (#l0 #l1 #h0 #h1:Type0)
+  (r0:rel l0 h0) 
+  (r1:rel l1 h1)
+  (xl: (l0 & l1))
+  (xh: erased (h0 & h1)) (res:slprop)
+requires 
+  rel_pair r0 r1 xl xh **
+  Trade.trade (rel_pair r0 r1 xl xh) res
+returns v:l0
+ensures 
+  r0 v (fst xh) ** 
+  Trade.trade (r0 v (fst xh)) res **
+  pure (v == fst xl)
+{
+  let f, s = destruct_pair_concrete _ _ _ _ _;
+  Trade.Util.elim_hyp_r _ _ res;
+  fst (f, s)
+}
+
+fn snd_pair_concrete (#l0 #l1 #h0 #h1:Type0)
+  (r0:rel l0 h0) 
+  (r1:rel l1 h1)
+  (xl: (l0 & l1))
+  (xh: erased (h0 & h1)) (res:slprop)
+requires 
+  rel_pair r0 r1 xl xh **
+  Trade.trade (rel_pair r0 r1 xl xh) res
+returns v:l1
+ensures 
+  r1 v (snd xh) ** 
+  Trade.trade (r1 v (snd xh)) res **
+  pure (v == snd xl)
+{
+  let f, s = destruct_pair_concrete _ _ _ _ _;
+  Trade.Util.elim_hyp_l _ _ res;
+  snd (f, s)
+}
+
+let is_derive_context_input
+    (res:option (either engine_record_t derive_context_l0_record_t))
+    (dflt:slprop) =
+  match res with
+  | None -> dflt
+  | Some e -> is_derive_context_input_args e dflt
+
+ghost
+fn trans_is_derive_context_input_args
+     e res res'
+requires is_derive_context_input_args e res ** Trade.trade res res'
+ensures is_derive_context_input_args e res'
+{
+  unfold is_derive_context_input_args;
+  match e {
+    Inl e -> {
+      assert (is_engine_record e res);
+      is_engine_record_compose e res res';
+      fold (is_derive_context_input_args (Inl e));
+    }
+    Inr e -> {
+      assert (is_derive_context_l0_record e res);
+      is_derive_context_l0_record_compose e res res';
+      fold (is_derive_context_input_args (Inr e));
+    }
+  }
+}
+
+fn extract_option_derive_context_input_args_data x (w:erased _) res
+requires rel_option (rel_evercddl_derive_context_input_args_data) x w **
+         Trade.trade (rel_option (rel_evercddl_derive_context_input_args_data) x w)
+                      res
+returns e:option (either engine_record_t derive_context_l0_record_t)
+ensures is_derive_context_input e res
+{
+  rel_option_cases _ _ _;
+  match x {
+    None -> {
+      Trade.elim_trade _ _;
+      fold (is_derive_context_input None res);
+      None    
+    }
+    Some x -> {
+     let xx = destruct_rel_option _ _ _;
+     Trade.trade_compose _ _ res;
+     let ret = extract_derive_context_input_args_data _ _;
+     trans_is_derive_context_input_args _ _ _;
+     fold (is_derive_context_input (Some ret) res);
+     Some ret
+    }
+  }
+}
+
+fn extract_derive_context_input_args x (w:erased _)
+requires rel_evercddl_derive_context_input_args x w
+returns e:option (either engine_record_t derive_context_l0_record_t)
+ensures is_derive_context_input e (rel_evercddl_derive_context_input_args x w)
+{
+  unfold_with_trade
+    (`%rel_evercddl_derive_context_input_args) 
+    (rel_evercddl_derive_context_input_args x w);
+  destruct_rel_fun _ _ _ _ _;
+  Trade.trade_compose _ _ (rel_evercddl_derive_context_input_args x w);
+  fold_last_relation (`%tstr_any) tstr_any;  
+  let rest_12 = fst_pair_concrete _ _ _ _ _;
+  let rest_11 = fst_pair_concrete _ _ _ _ _;
+  let rest_10 = fst_pair_concrete _ _ _ _ _;
+  let rest_9 = fst_pair_concrete _ _ _ _ _;
+  let rest_8 = fst_pair_concrete _ _ _ _ _;
+  let rest_7 = fst_pair_concrete _ _ _ _ _;
+  let rest_6 = fst_pair_concrete _ _ _ _ _;
+  let input_data = snd_pair_concrete _ _ _ _ _;
+  rewrite each  
+    (Tactics.PrettifyType.named "intkey6"
+          evercddl_derive_context_input_args_data_pretty)
+  as evercddl_derive_context_input_args_data_pretty;
+  extract_option_derive_context_input_args_data _ _ _;
+}
+
+ghost
+fn trans_is_derive_context_input
+     e res res'
+requires is_derive_context_input e res ** Trade.trade res res'
+ensures is_derive_context_input e res'
+{
+  unfold is_derive_context_input;
+  match e {
+    None -> {
+      Trade.elim_trade _ _;
+      fold (is_derive_context_input None res');
+    }
+    Some e -> {
+      assert (is_derive_context_input_args e res);
+      trans_is_derive_context_input_args e res res';
+      fold (is_derive_context_input (Some e) res');
+    }
+  }
+}
+
 
 fn parse_derive_context_input_args (s:Slice.slice UInt8.t) (#p:perm) (#w:erased _)
 requires pts_to s #p w
-returns x:option (slice UInt8.t) //todo, check that slice_len is uds_len
-ensures pts_to s #p w
+returns e:option (either engine_record_t derive_context_l0_record_t)
+ensures is_derive_context_input e (pts_to s #p w)
 {
   let res = validate_and_parse_derive_context_input_args s;
   match res {
     None -> {
       unfold validate_and_parse_post;
+      fold (is_derive_context_input None (pts_to s #p w));
       None
     }
     Some xrem -> {
       let (x, rem) = xrem;
       elim_validate_and_parse_post_some x rem;
-      extract_devive_context_input_args x _;
-      admit()
+      let res = extract_derive_context_input_args x _;
+      Trade.Util.elim_hyp_r _ _ _;
+      trans_is_derive_context_input _ _ _;
+      res
     }
   }
 }
